new theorems

Lambda/Defs.lean
@@ -18,35 +18,175 @@ instance : ToString Lambda := ⟨Lambda.toString⟩
 instance : Repr Lambda where
   reprPrec M _ := M.toString.toFormat
 
-def Lambda.shift (c : Nat) (i : Int) : Lambda → Lambda
+def Lambda.shift (c : Nat) (i : Nat) : Lambda → Lambda
   | var n =>
     if n < c then var n
-    else var (n + i).toNat
+    else var (n + i)
   | app e₁ e₂ => app (e₁.shift c i) (e₂.shift c i)
   | abs e => abs (e.shift (c + 1) i)
 
+
+notation:60 "↑"  c:61  i:62  t:63 => Lambda.shift c i t
+
 def Lambda.subst (v : Lambda) (e : Lambda) (m : Nat) : Lambda :=
   match v with
-  | var n => if n = m then e else var n
+  | var n =>
+    if n < m then var n
+    else if n = m then e.shift 0 m
+    else var (n - 1)
   | app v₁ v₂ => app (v₁.subst e m) (v₂.subst e m)
-  | abs v₁ => abs $ v₁.subst (e.shift 0 1) (m + 1)
+  | abs v₁ => abs $ v₁.subst e (m + 1)
+
+notation:65 t:65 "[" k " ↦ " s:65 "]" => Lambda.subst t s k
 
 def Redex (e : Lambda) := ∃ (e₁ e₂ : Lambda), e = (λ e₁).app e₂
 
-def Lambda.beta : Lambda → Lambda
-  | app e₁ e₂ =>
-    match e₁ with
-    | abs v => (v.subst (e₂.shift 0 1) 0).shift 0 (-1)
-    | _ => app e₁ e₂
-  | e => e
+-- def Lambda.beta : Lambda → Lambda
+--   | app e₁ e₂ =>
+--     match e₁ with
+--     | abs v => (v.subst (e₂.shift 0 1) 0).shift 0 (-1)
+--     | _ => app e₁ e₂
+--   | e => e
 
-inductive BetaR : Lambda → Lambda → Prop
-| basis (M : Lambda) : BetaR M M.beta
-| app_left (M N L) : BetaR M N → BetaR (.app M L) (.app N L)
-| app_right (M N L) : BetaR M N → BetaR (.app L M) (.app L N)
-| abs (M N) : BetaR M N → BetaR (λ M) (λ N)
-| refl (M) : BetaR M M
+-- inductive BetaR : Lambda → Lambda → Prop
+--   | basis (M : Lambda) : BetaR M M.beta
+--   | app_left (M N L) : BetaR M N → BetaR (.app M L) (.app N L)
+--   | app_right (M N L) : BetaR M N → BetaR (.app L M) (.app L N)
+--   | abs (M N) : BetaR M N → BetaR (λ M) (λ N)
+--   | refl (M) : BetaR M M
 
-inductive BetaRR : Lambda → Lambda → Prop
-| beta (M N) : BetaR M N → BetaRR M N
-| trans (M N L) : BetaRR M N → BetaRR N L → BetaRR M L
+-- inductive BetaRR : Lambda → Lambda → Prop
+--   | beta (M N) : BetaR M N → BetaRR M N
+--   | trans (M N L) : BetaRR M N → BetaRR N L → BetaRR M L
+
+
+theorem sustitution_lem1 (n m : Nat) (N : Lambda)
+  : ∀ (i j : Nat), i ≤ j → j ≤ i + m → (N.shift i m).shift j n = N.shift i (m + n)
+  := by
+  induction N with
+  | var k =>
+    intro i j ilej jlem1
+    simp_all [Lambda.shift]
+    rcases Nat.lt_trichotomy k i with klei | rfl | kgti
+    . simp [klei]
+      rw [Lambda.shift]
+      simp [Nat.lt_of_lt_of_le klei ilej]
+    . simp
+      rw [Lambda.shift]
+      simp [Nat.not_lt.mpr jlem1]
+      rw [Nat.add_assoc]
+    . simp [Nat.not_lt_of_gt kgti]
+      rw [Lambda.shift]
+      have : i + m < k + m := by exact Nat.add_lt_add_right kgti m
+      have : j < k + m := by exact Nat.lt_of_le_of_lt jlem1 this
+      simp [Nat.not_lt_of_gt this]
+      rw [Nat.add_assoc]
+  | app e v ihe ihv =>
+    intro i j ilej jlemi
+    simp_all [Lambda.shift]
+  | abs e ih =>
+    intro i j ilej jleim
+    simp_all [Lambda.shift]
+    apply ih
+    exact Nat.add_le_add_right ilej 1
+    rw [Nat.add_assoc, Nat.add_comm 1 m, ← Nat.add_assoc]
+    exact Nat.add_le_add_right jleim 1
+
+theorem sustitution_lem2 (i : Nat) (N L : Lambda)
+  : ∀ (k j : Nat), k ≤ j → (N[j ↦ L]).shift k i = (N.shift k i)[j + i ↦ L] := by
+  induction N with
+  | var n =>
+    intro k j klej
+    rcases Nat.lt_trichotomy n k with nlek | rfl | ngtk
+    . have nlej : n < j := Nat.lt_of_lt_of_le nlek klej
+      have nleji : n < j + i := Nat.lt_add_right i nlej
+      simp [Lambda.shift, Lambda.subst, nlek, nleji, nlej]
+    . rcases Or.symm (Nat.eq_or_lt_of_le klej) with nlej | rfl
+      . simp [Lambda.subst, Lambda.shift, nlej]
+      . simp_all [Lambda.subst, Lambda.shift]
+        apply sustitution_lem1 <;> simp
+    . rcases Nat.lt_trichotomy n j with nlej | rfl | ngtj
+      . simp [Lambda.subst, Lambda.shift, Nat.not_lt_of_gt ngtk, nlej]
+      . simp [Lambda.subst, Lambda.shift, Nat.not_lt_of_gt ngtk]
+        apply sustitution_lem1 <;> simp [klej]
+      .
+        have : ¬ (n - 1 < k) := by
+          intro h
+          apply Nat.lt_irrefl (n - 1)
+          apply Nat.lt_of_lt_of_le h
+          exact Nat.le_sub_one_of_lt ngtk
+        simp [
+          Lambda.subst,
+          Lambda.shift,
+          Nat.not_lt_of_gt ngtj,
+          Ne.symm (Nat.ne_of_lt ngtj),
+          this,
+          Nat.not_lt_of_gt ngtk
+        ]
+        rw [Nat.sub_add_comm]
+        exact (Nat.zero_lt_of_lt ngtk)
+  | app e v ihe ihv =>
+    intro i j ilej
+    simp_all [Lambda.shift, Lambda.subst]
+  | abs e ihe =>
+    intro k j ilej
+    simp_all [Lambda.subst, Lambda.shift]
+    rw [Nat.add_assoc, Nat.add_comm 1 i, ← Nat.add_assoc]
+
+theorem sustitution (n m : Nat) (nlem : n ≤ m) (M N L : Lambda)
+  : M[n ↦ N][m ↦ L] = M[m + 1 ↦ L][n ↦ N[m - n ↦ L]] := by
+  induction M with
+  | var k =>
+    rcases Nat.lt_trichotomy k n with klen | rfl | kgtn
+    -- Case k < n
+    . rw [Lambda.subst, Lambda.subst]
+      have klem1 : k < m + 1 := by
+        apply Nat.lt_of_lt_of_le
+        exact klen
+        exact Nat.le_add_right_of_le nlem
+      have klem : k < m := by exact Nat.lt_of_lt_of_le klen nlem
+      simp [klen, klem1]
+      rw [Lambda.subst, Lambda.subst]
+      simp [klem, klen]
+    -- Case k = n
+    . rw [Lambda.subst]
+      simp
+      have klem1 : k < m + 1 := by exact Nat.lt_add_one_of_le nlem
+      rw [Lambda.subst]
+      simp [klem1]
+      rw [Lambda.subst]
+      simp
+      have zero_le_mmk : 0 ≤ m - k := (Nat.le_sub_iff_add_le' nlem).mpr nlem
+      rw [eq_comm]
+      have := by
+        apply sustitution_lem2 k N L
+        exact zero_le_mmk
+      simp [Nat.sub_add_cancel nlem] at this
+      assumption
+    -- case n < k
+    .
+      have (h₁ : 0 < k) : k - 1 < m ↔ k < m + 1 := by
+        conv =>
+          lhs
+          rw [← Nat.add_lt_add_iff_right, Nat.sub_add_cancel h₁]
+          simp
+      simp [
+        Lambda.subst,
+        Nat.not_lt_of_gt kgtn,
+        Ne.symm (Nat.ne_of_lt kgtn)
+      ]
+      simp [this <| Nat.zero_lt_of_lt kgtn]
+      rcases Nat.lt_trichotomy k (m + 1) with kltm1 | rfl | kgtm1
+      . simp [
+          kltm1,
+          Lambda.subst,
+          Nat.not_lt_of_gt kgtn,
+          Ne.symm (Nat.ne_of_lt kgtn)
+        ]
+      . sorry
+      .
+
+
+
+
+#check sustitution_lem2
